tests/test.bpl
@@ -1,9 +1,9 @@
 // 
 // Translation of Viper program.
 // 
-// Date:         2021-03-19 23:28:15
+// Date:         2021-04-09 17:41:45
 // Tool:         carbon 1.0
-// Arguments: :  --z3Exe /usr/bin/z3 --boogieExe /bin/boogie/Binaries/boogie --print tests/test.bpl tests/predicate_test.vpr
+// Arguments: :  --z3Exe /usr/bin/z3 --boogieExe /bin/boogie/Binaries/boogie --translateOnly --print tests/test.bpl tests/test.vpr
 // Dependencies:
 //   Boogie , located at /bin/boogie/Binaries/boogie.
 //   Z3 4.8.4 - 64 bit, located at /usr/bin/z3.
@@ -144,6 +144,24 @@ axiom (forall <A, B> ResultMask: MaskType, SummandMask1: MaskType, SummandMask2:
   { sumMask(ResultMask, SummandMask1, SummandMask2), ResultMask[o_1, f_3] } { sumMask(ResultMask, SummandMask1, SummandMask2), SummandMask1[o_1, f_3] } { sumMask(ResultMask, SummandMask1, SummandMask2), SummandMask2[o_1, f_3] }
   sumMask(ResultMask, SummandMask1, SummandMask2) ==> ResultMask[o_1, f_3] == SummandMask1[o_1, f_3] + SummandMask2[o_1, f_3]
 );
+// ==================================================
+// Function for trigger used in checks which are never triggered
+// ==================================================
+
+function  neverTriggered1(r_1: Ref): bool;
+function  neverTriggered2(r_3: Ref): bool;
+// ==================================================
+// Functions used as inverse of receiver expressions in quantified permissions during inhale and exhale
+// ==================================================
+
+function  invRecv1(recv: Ref): Ref;
+function  invRecv2(recv: Ref): Ref;
+// ==================================================
+// Functions used to represent the range of the projection of each QP instance onto its receiver expressions for quantified permissions during inhale and exhale
+// ==================================================
+
+function  qpRange1(recv: Ref): bool;
+function  qpRange2(recv: Ref): bool;
 
 // ==================================================
 // Preamble of Function and predicate module.
@@ -178,6 +196,197 @@ axiom (forall <A> p: (Field A FrameType), v_1: FrameType, w: FrameType ::
 );
 
 // ==================================================
+// Preamble of Set module.
+// ==================================================
+
+
+type Set T = [T]bool;
+
+function Set#Card<T>(Set T): int;
+axiom (forall<T> s: Set T :: { Set#Card(s) } 0 <= Set#Card(s));
+
+function Set#Empty<T>(): Set T;
+axiom (forall<T> o: T :: { Set#Empty()[o] } !Set#Empty()[o]);
+axiom (forall<T> s: Set T :: { Set#Card(s) }
+  (Set#Card(s) == 0 <==> s == Set#Empty()) &&
+  (Set#Card(s) != 0 ==> (exists x: T :: s[x])));
+
+function Set#Singleton<T>(T): Set T;
+axiom (forall<T> r: T :: { Set#Singleton(r) } Set#Singleton(r)[r]);
+axiom (forall<T> r: T, o: T :: { Set#Singleton(r)[o] } Set#Singleton(r)[o] <==> r == o);
+axiom (forall<T> r: T :: { Set#Card(Set#Singleton(r)) } Set#Card(Set#Singleton(r)) == 1);
+
+function Set#UnionOne<T>(Set T, T): Set T;
+axiom (forall<T> a: Set T, x: T, o: T :: { Set#UnionOne(a,x)[o] }
+  Set#UnionOne(a,x)[o] <==> o == x || a[o]);
+axiom (forall<T> a: Set T, x: T :: { Set#UnionOne(a, x) }
+  Set#UnionOne(a, x)[x]);
+axiom (forall<T> a: Set T, x: T, y: T :: { Set#UnionOne(a, x), a[y] }
+  a[y] ==> Set#UnionOne(a, x)[y]);
+axiom (forall<T> a: Set T, x: T :: { Set#Card(Set#UnionOne(a, x)) }
+  a[x] ==> Set#Card(Set#UnionOne(a, x)) == Set#Card(a));
+axiom (forall<T> a: Set T, x: T :: { Set#Card(Set#UnionOne(a, x)) }
+  !a[x] ==> Set#Card(Set#UnionOne(a, x)) == Set#Card(a) + 1);
+
+function Set#Union<T>(Set T, Set T): Set T;
+axiom (forall<T> a: Set T, b: Set T, o: T :: { Set#Union(a,b)[o] }
+  Set#Union(a,b)[o] <==> a[o] || b[o]);
+axiom (forall<T> a, b: Set T, y: T :: { Set#Union(a, b), a[y] }
+  a[y] ==> Set#Union(a, b)[y]);
+axiom (forall<T> a, b: Set T, y: T :: { Set#Union(a, b), b[y] }
+  b[y] ==> Set#Union(a, b)[y]);
+//axiom (forall<T> a, b: Set T :: { Set#Union(a, b) }
+//  Set#Disjoint(a, b) ==>
+//    Set#Difference(Set#Union(a, b), a) == b &&
+//    Set#Difference(Set#Union(a, b), b) == a);
+
+function Set#Intersection<T>(Set T, Set T): Set T;
+axiom (forall<T> a: Set T, b: Set T, o: T :: { Set#Intersection(a,b)[o] } {Set#Intersection(a,b), a[o]} {Set#Intersection(a,b), b[o]} // AS: added alternative triggers 20/06/19
+  Set#Intersection(a,b)[o] <==> a[o] && b[o]);
+
+axiom (forall<T> a, b: Set T :: { Set#Union(Set#Union(a, b), b) }
+  Set#Union(Set#Union(a, b), b) == Set#Union(a, b));
+axiom (forall<T> a, b: Set T :: { Set#Union(a, Set#Union(a, b)) }
+  Set#Union(a, Set#Union(a, b)) == Set#Union(a, b));
+axiom (forall<T> a, b: Set T :: { Set#Intersection(Set#Intersection(a, b), b) }
+  Set#Intersection(Set#Intersection(a, b), b) == Set#Intersection(a, b));
+axiom (forall<T> a, b: Set T :: { Set#Intersection(a, Set#Intersection(a, b)) }
+  Set#Intersection(a, Set#Intersection(a, b)) == Set#Intersection(a, b));
+axiom (forall<T> a, b: Set T :: { Set#Card(Set#Union(a, b)) }{ Set#Card(Set#Intersection(a, b)) }
+  Set#Card(Set#Union(a, b)) + Set#Card(Set#Intersection(a, b)) == Set#Card(a) + Set#Card(b));
+
+function Set#Difference<T>(Set T, Set T): Set T;
+axiom (forall<T> a: Set T, b: Set T, o: T :: { Set#Difference(a,b)[o] } { Set#Difference(a,b), a[o] }
+  Set#Difference(a,b)[o] <==> a[o] && !b[o]);
+axiom (forall<T> a, b: Set T, y: T :: { Set#Difference(a, b), b[y] }
+  b[y] ==> !Set#Difference(a, b)[y] );
+axiom (forall<T> a, b: Set T ::
+  { Set#Card(Set#Difference(a, b)) }
+  Set#Card(Set#Difference(a, b)) + Set#Card(Set#Difference(b, a))
+  + Set#Card(Set#Intersection(a, b))
+    == Set#Card(Set#Union(a, b)) &&
+  Set#Card(Set#Difference(a, b)) == Set#Card(a) - Set#Card(Set#Intersection(a, b)));
+
+function Set#Subset<T>(Set T, Set T): bool;
+axiom(forall<T> a: Set T, b: Set T :: { Set#Subset(a,b) }
+  Set#Subset(a,b) <==> (forall o: T :: {a[o]} {b[o]} a[o] ==> b[o]));
+// axiom(forall<T> a: Set T, b: Set T ::
+//   { Set#Subset(a,b), Set#Card(a), Set#Card(b) }  // very restrictive trigger
+//   Set#Subset(a,b) ==> Set#Card(a) <= Set#Card(b));
+
+
+function Set#Equal<T>(Set T, Set T): bool;
+axiom(forall<T> a: Set T, b: Set T :: { Set#Equal(a,b) }
+  Set#Equal(a,b) <==> (forall o: T :: {a[o]} {b[o]} a[o] <==> b[o]));
+axiom(forall<T> a: Set T, b: Set T :: { Set#Equal(a,b) }  // extensionality axiom for sets
+  Set#Equal(a,b) ==> a == b);
+
+//function Set#Disjoint<T>(Set T, Set T): bool;
+//axiom (forall<T> a: Set T, b: Set T :: { Set#Disjoint(a,b) }
+//  Set#Disjoint(a,b) <==> (forall o: T :: {a[o]} {b[o]} !a[o] || !b[o]));
+
+// ---------------------------------------------------------------
+// -- Axiomatization of multisets --------------------------------
+// ---------------------------------------------------------------
+
+function Math#min(a: int, b: int): int;
+axiom (forall a: int, b: int :: { Math#min(a, b) } a <= b <==> Math#min(a, b) == a);
+axiom (forall a: int, b: int :: { Math#min(a, b) } b <= a <==> Math#min(a, b) == b);
+axiom (forall a: int, b: int :: { Math#min(a, b) } Math#min(a, b) == a || Math#min(a, b) == b);
+
+function Math#clip(a: int): int;
+axiom (forall a: int :: { Math#clip(a) } 0 <= a ==> Math#clip(a) == a);
+axiom (forall a: int :: { Math#clip(a) } a < 0  ==> Math#clip(a) == 0);
+
+type MultiSet T; // = [T]int;
+
+function MultiSet#Select<T>(ms: MultiSet T, x:T): int;
+
+//function $IsGoodMultiSet<T>(ms: MultiSet T): bool;
+// ints are non-negative, used after havocing, and for conversion from sequences to multisets.
+//axiom (forall<T> ms: MultiSet T :: { $IsGoodMultiSet(ms) }
+//  $IsGoodMultiSet(ms) <==>
+//  (forall bx: T :: { ms[bx] } 0 <= ms[bx] && ms[bx] <= MultiSet#Card(ms)));
+
+axiom (forall<T> ms: MultiSet T, x: T :: {MultiSet#Select(ms,x)} MultiSet#Select(ms,x) >= 0); // NEW
+
+function MultiSet#Card<T>(MultiSet T): int;
+axiom (forall<T> s: MultiSet T :: { MultiSet#Card(s) } 0 <= MultiSet#Card(s));
+//axiom (forall<T> s: MultiSet T, x: T, n: int :: { MultiSet#Card(s[x := n]) }
+//  0 <= n ==> MultiSet#Card(s[x := n]) == MultiSet#Card(s) - s[x] + n);
+//
+function MultiSet#Empty<T>(): MultiSet T;
+axiom (forall<T> o: T :: { MultiSet#Select(MultiSet#Empty(),o) } MultiSet#Select(MultiSet#Empty(),o) == 0);
+axiom (forall<T> s: MultiSet T :: { MultiSet#Card(s) }
+  (MultiSet#Card(s) == 0 <==> s == MultiSet#Empty()) &&
+  (MultiSet#Card(s) != 0 ==> (exists x: T :: 0 < MultiSet#Select(s,x))));
+
+function MultiSet#Singleton<T>(T): MultiSet T;
+axiom (forall<T> r: T, o: T :: { MultiSet#Select(MultiSet#Singleton(r),o) } (MultiSet#Select(MultiSet#Singleton(r),o) == 1 <==> r == o) &&
+                                                            (MultiSet#Select(MultiSet#Singleton(r),o) == 0 <==> r != o));
+axiom (forall<T> r: T :: { MultiSet#Singleton(r) } MultiSet#Card(MultiSet#Singleton(r)) == 1 && MultiSet#Select(MultiSet#Singleton(r),r) == 1); // AS: added
+axiom (forall<T> r: T :: { MultiSet#Singleton(r) } MultiSet#Singleton(r) == MultiSet#UnionOne(MultiSet#Empty(), r)); // AS: remove this?
+
+function MultiSet#UnionOne<T>(MultiSet T, T): MultiSet T;
+// union-ing increases count by one for x, not for others
+axiom (forall<T> a: MultiSet T, x: T, o: T :: { MultiSet#Select(MultiSet#UnionOne(a,x),o) } { MultiSet#UnionOne(a, x), MultiSet#Select(a,o) } // AS: added back this trigger (used on a similar axiom before)
+  MultiSet#Select(MultiSet#UnionOne(a, x),o) == (if x==o then MultiSet#Select(a,o) + 1 else MultiSet#Select(a,o)));
+// non-decreasing
+axiom (forall<T> a: MultiSet T, x: T :: { MultiSet#Card(MultiSet#UnionOne(a, x)) } {MultiSet#UnionOne(a, x), MultiSet#Card(a)} // AS: added alternative trigger
+  MultiSet#Card(MultiSet#UnionOne(a, x)) == MultiSet#Card(a) + 1);
+// AS: added - concrete knowledge of element added
+axiom (forall<T> a: MultiSet T, x: T :: { MultiSet#UnionOne(a,x)}
+  MultiSet#Select(MultiSet#UnionOne(a, x),x) > 0 && MultiSet#Card(MultiSet#UnionOne(a, x)) > 0);
+
+function MultiSet#Union<T>(MultiSet T, MultiSet T): MultiSet T;
+// union-ing is the sum of the contents
+axiom (forall<T> a: MultiSet T, b: MultiSet T, o: T :: { MultiSet#Select(MultiSet#Union(a,b),o) } {MultiSet#Union(a,b), MultiSet#Select(a,o), MultiSet#Select(b,o)}// AS: added triggers
+  MultiSet#Select(MultiSet#Union(a,b),o) == MultiSet#Select(a,o) + MultiSet#Select(b,o));
+axiom (forall<T> a: MultiSet T, b: MultiSet T :: { MultiSet#Card(MultiSet#Union(a,b)) } {MultiSet#Card(a), MultiSet#Union(a,b)} {MultiSet#Card(b), MultiSet#Union(a,b)}
+  MultiSet#Card(MultiSet#Union(a,b)) == MultiSet#Card(a) + MultiSet#Card(b));
+
+function MultiSet#Intersection<T>(MultiSet T, MultiSet T): MultiSet T;
+axiom (forall<T> a: MultiSet T, b: MultiSet T, o: T :: { MultiSet#Select(MultiSet#Intersection(a,b),o) }
+  MultiSet#Select(MultiSet#Intersection(a,b),o) == Math#min(MultiSet#Select(a,o),  MultiSet#Select(b,o)));
+
+// left and right pseudo-idempotence
+axiom (forall<T> a, b: MultiSet T :: { MultiSet#Intersection(MultiSet#Intersection(a, b), b) }
+  MultiSet#Intersection(MultiSet#Intersection(a, b), b) == MultiSet#Intersection(a, b));
+axiom (forall<T> a, b: MultiSet T :: { MultiSet#Intersection(a, MultiSet#Intersection(a, b)) }
+  MultiSet#Intersection(a, MultiSet#Intersection(a, b)) == MultiSet#Intersection(a, b));
+
+// multiset difference, a - b. clip() makes it positive.
+function MultiSet#Difference<T>(MultiSet T, MultiSet T): MultiSet T;
+axiom (forall<T> a: MultiSet T, b: MultiSet T, o: T :: { MultiSet#Select(MultiSet#Difference(a,b),o) }
+  MultiSet#Select(MultiSet#Difference(a,b),o) == Math#clip(MultiSet#Select(a,o) - MultiSet#Select(b,o)));
+axiom (forall<T> a, b: MultiSet T, y: T :: { MultiSet#Difference(a, b), MultiSet#Select(b,y), MultiSet#Select(a,y) }
+  MultiSet#Select(a,y) <= MultiSet#Select(b,y) ==> MultiSet#Select(MultiSet#Difference(a, b),y) == 0 );
+axiom (forall<T> a, b: MultiSet T ::
+  { MultiSet#Card(MultiSet#Difference(a, b)) }
+  MultiSet#Card(MultiSet#Difference(a, b)) + MultiSet#Card(MultiSet#Difference(b, a))
+  + 2 * MultiSet#Card(MultiSet#Intersection(a, b))
+    == MultiSet#Card(MultiSet#Union(a, b)) &&
+  MultiSet#Card(MultiSet#Difference(a, b)) == MultiSet#Card(a) - MultiSet#Card(MultiSet#Intersection(a, b)));
+
+// multiset subset means a must have at most as many of each element as b
+function MultiSet#Subset<T>(MultiSet T, MultiSet T): bool;
+axiom(forall<T> a: MultiSet T, b: MultiSet T :: { MultiSet#Subset(a,b) }
+  MultiSet#Subset(a,b) <==> (forall o: T :: {MultiSet#Select(a,o)} {MultiSet#Select(b,o)} MultiSet#Select(a,o) <= MultiSet#Select(b,o)));
+
+function MultiSet#Equal<T>(MultiSet T, MultiSet T): bool;
+axiom(forall<T> a: MultiSet T, b: MultiSet T :: { MultiSet#Equal(a,b) }
+  MultiSet#Equal(a,b) <==> (forall o: T :: {MultiSet#Select(a,o)} {MultiSet#Select(b,o)} MultiSet#Select(a,o) == MultiSet#Select(b,o)));
+// extensionality axiom for multisets
+axiom(forall<T> a: MultiSet T, b: MultiSet T :: { MultiSet#Equal(a,b) }
+  MultiSet#Equal(a,b) ==> a == b);
+
+function MultiSet#Disjoint<T>(MultiSet T, MultiSet T): bool;
+axiom (forall<T> a: MultiSet T, b: MultiSet T :: { MultiSet#Disjoint(a,b) }
+  MultiSet#Disjoint(a,b) <==> (forall o: T :: {MultiSet#Select(a,o)} {MultiSet#Select(b,o)} MultiSet#Select(a,o) == 0 || MultiSet#Select(b,o) == 0));
+
+    
+
+// ==================================================
 // Translation of all fields
 // ==================================================
 
@@ -186,66 +395,22 @@ axiom !IsPredicateField(f_6);
 axiom !IsWandField(f_6);
 
 // ==================================================
-// Translation of predicate foo
+// Translation of method main
 // ==================================================
 
-type PredicateType_foo;
-function  foo(xs: Ref): Field PredicateType_foo FrameType;
-function  foo#sm(xs: Ref): Field PredicateType_foo PMaskType;
-axiom (forall xs: Ref ::
-  { PredicateMaskField(foo(xs)) }
-  PredicateMaskField(foo(xs)) == foo#sm(xs)
-);
-axiom (forall xs: Ref ::
-  { foo(xs) }
-  IsPredicateField(foo(xs))
-);
-axiom (forall xs: Ref ::
-  { foo(xs) }
-  getPredicateId(foo(xs)) == 0
-);
-function  foo#trigger<A>(Heap: HeapType, pred: (Field A FrameType)): bool;
-function  foo#everUsed<A>(pred: (Field A FrameType)): bool;
-axiom (forall xs: Ref, xs2: Ref ::
-  { foo(xs), foo(xs2) }
-  foo(xs) == foo(xs2) ==> xs == xs2
-);
-axiom (forall xs: Ref, xs2: Ref ::
-  { foo#sm(xs), foo#sm(xs2) }
-  foo#sm(xs) == foo#sm(xs2) ==> xs == xs2
-);
-
-axiom (forall Heap: HeapType, xs: Ref ::
-  { foo#trigger(Heap, foo(xs)) }
-  foo#everUsed(foo(xs))
-);
-
-// ==================================================
-// Translation of method test
-// ==================================================
-
-procedure test(x: Ref) returns ()
+procedure main(s: (Set Ref)) returns ()
   modifies Heap, Mask, BMask;
 {
-  var wildcard: real where wildcard > NoPerm;
-  var perm: Perm;
-  var newVersion: FrameType;
-  var v_2: int;
-  var freshVersion: FrameType;
+  var x: Ref;
+  var y: Ref;
+  var QPMask: MaskType;
+  var QPBMask: BMaskType;
+  var sWildcard: real;
+  var ExhaleHeap: HeapType;
   
   // -- Initializing the state
     Mask := ZeroMask;
     BMask := ZeroBMask;
-    assume state(Heap, Mask, BMask);
-  
-  // -- Assumptions about method arguments
-    assume Heap[x, $allocated];
-  
-  // -- Checked inhaling of precondition
-    havoc wildcard;
-    perm := wildcard;
-    Mask[null, foo(x)] := Mask[null, foo(x)] + perm;
-    assume state(Heap, Mask, BMask);
     assume state(Heap, Mask, BMask);
   
   // -- Initializing of old state
@@ -255,63 +420,123 @@ procedure test(x: Ref) returns ()
       assume Mask == old(Mask);
       assume BMask == old(BMask);
   
-  // -- Translating statement: unfold acc(foo(x), wildcard) -- predicate_test.vpr@11.19--12.5
-    assume foo#trigger(Heap, foo(x));
-    assume Heap[null, foo(x)] == FrameFragment(Heap[x, f_6]);
-    // Phase 1: pure assertions and fixed permissions
+  // -- Assumptions about local variables
+    assume Heap[x, $allocated];
+    assume Heap[y, $allocated];
+  
+  // -- Translating statement: inhale (forall r: Ref :: { (r in s) } (r in s) ==> acc(r.f, sWildcard)) -- test.vpr@5.11--7.5
     
-    // -- Update version of predicate
-      if (!HasDirectPerm(Mask, BMask, null, foo(x))) {
-        havoc newVersion;
-        Heap[null, foo(x)] := newVersion;
+    // -- Check definedness of (forall r: Ref :: { (r in s) } (r in s) ==> acc(r.f, sWildcard))
+      if (*) {
+        assume false;
       }
-    // Phase 3: all remaining permissions (containing read permissions, but in a negative context)
-    perm := NoPerm;
-    havoc wildcard;
-    perm := perm + wildcard;
-    assert {:msg "  Unfolding foo(x) might fail. There might be insufficient permission to access foo(x) (predicate_test.vpr@11.19--12.5) [5]"}
-      Mask[null, foo(x)] > NoPerm || BMask[null, foo(x)];
-    assume wildcard < Mask[null, foo(x)];
-    Mask[null, foo(x)] := Mask[null, foo(x)] - perm;
-    havoc wildcard;
-    perm := wildcard;
-    assume x != null;
-    Mask[x, f_6] := Mask[x, f_6] + perm;
-    assume state(Heap, Mask, BMask);
-    assume state(Heap, Mask, BMask);
-    assume state(Heap, Mask, BMask);
-  
-  // -- Translating statement: v := x.f -- predicate_test.vpr@12.8--13.5
-    
-    // -- Check definedness of x.f
-      assert {:msg "  Assignment might fail. There might be insufficient permission to access x.f (predicate_test.vpr@12.8--13.5) [6]"}
-        HasDirectPerm(Mask, BMask, x, f_6);
       assume state(Heap, Mask, BMask);
-    v_2 := Heap[x, f_6];
+    havoc QPMask;
+    havoc QPBMask;
+    
+    // -- Define Inverse Function
+      assume (forall r_1: Ref ::
+        { Heap[r_1, f_6] } { QPMask[r_1, f_6] } { s[r_1] }
+        s[r_1] ==> qpRange1(r_1) && invRecv1(r_1) == r_1
+      );
+      assume (forall o_2: Ref ::
+        { invRecv1(o_2) }
+        s[invRecv1(o_2)] && qpRange1(o_2) ==> invRecv1(o_2) == o_2
+      );
+    
+    // -- Assume set of fields is nonNull
+      assume (forall r_1: Ref ::
+        { Heap[r_1, f_6] } { QPMask[r_1, f_6] } { s[r_1] }
+        s[r_1] ==> r_1 != null
+      );
+    
+    // -- Define permissions
+      assume (forall o_2: Ref ::
+        { QPMask[o_2, f_6] } { QPBMask[o_2, f_6] }
+        (s[invRecv1(o_2)] && qpRange1(o_2) ==> invRecv1(o_2) == o_2 && (QPMask[o_2, f_6] == Mask[o_2, f_6] && QPBMask[o_2, f_6])) && (!(s[invRecv1(o_2)] && qpRange1(o_2)) ==> QPMask[o_2, f_6] == Mask[o_2, f_6] && QPBMask[o_2, f_6] == BMask[o_2, f_6])
+      );
+      assume (forall <A, B> o_2: Ref, f_4: (Field A B) ::
+        { Mask[o_2, f_4] } { QPMask[o_2, f_4] }
+        f_4 != f_6 ==> Mask[o_2, f_4] == QPMask[o_2, f_4] && BMask[o_2, f_4] == QPBMask[o_2, f_4]
+      );
+    Mask := QPMask;
+    BMask := QPBMask;
+    assume state(Heap, Mask, BMask);
+    assume state(Heap, Mask, BMask);
     assume state(Heap, Mask, BMask);
   
-  // -- Translating statement: fold acc(foo(x), wildcard) -- predicate_test.vpr@13.17--14.1
-    // Phase 3: all remaining permissions (containing read permissions, but in a negative context)
-    perm := NoPerm;
-    havoc wildcard;
-    perm := perm + wildcard;
-    assert {:msg "  Folding foo(x) might fail. There might be insufficient permission to access x.f (predicate_test.vpr@13.17--14.1) [7]"}
-      Mask[x, f_6] > NoPerm || BMask[x, f_6];
-    assume wildcard < Mask[x, f_6];
-    Mask[x, f_6] := Mask[x, f_6] - perm;
-    havoc wildcard;
-    perm := wildcard;
-    Mask[null, foo(x)] := Mask[null, foo(x)] + perm;
+  // -- Translating statement: inhale (x in s) -- test.vpr@10.13--11.5
+    assume s[x];
     assume state(Heap, Mask, BMask);
     assume state(Heap, Mask, BMask);
-    assume foo#trigger(Heap, foo(x));
-    assume Heap[null, foo(x)] == FrameFragment(Heap[x, f_6]);
-    if (!HasDirectPerm(Mask, BMask, null, foo(x))) {
-      Heap[null, foo#sm(x)] := ZeroPMask;
-      havoc freshVersion;
-      Heap[null, foo(x)] := freshVersion;
-    }
-    Heap[null, foo#sm(x)][x, f_6] := true;
+  
+  // -- Translating statement: inhale (y in s) -- test.vpr@11.13--12.5
+    assume s[y];
     assume state(Heap, Mask, BMask);
+    assume state(Heap, Mask, BMask);
+  
+  // -- Translating statement: inhale x != y -- test.vpr@12.13--14.5
+    assume x != y;
+    assume state(Heap, Mask, BMask);
+    assume state(Heap, Mask, BMask);
+  
+  // -- Translating statement: exhale (forall r: Ref :: { (r in s) } (r in s) ==> acc(r.f, sWildcard)) -- test.vpr@14.11--14.12
+    
+    // -- Check definedness of (forall r: Ref :: { (r in s) } (r in s) ==> acc(r.f, sWildcard))
+      if (*) {
+        assume false;
+      }
+      assume state(Heap, Mask, BMask);
+    // Phase 1: pure assertions and fixed permissions
+    havoc QPMask;
+    havoc QPBMask;
+    // wild card assumptions
+    assert {:msg "  Exhale might fail. There might be insufficient permission to access r.f (test.vpr@14.11--14.12) [7]"}
+      (forall r_3: Ref ::
+      
+      s[r_3] ==> Mask[r_3, f_6] > NoPerm || BMask[r_3, f_6]
+    );
+    
+    // -- check if receiver r is injective
+      assert {:msg "  Exhale might fail. Receiver of r.f [test.vpr@14.57--14.57]  might not be injective. (test.vpr@14.11--14.12) [8]"}
+        (forall r_3: Ref, r_3_1: Ref ::
+        { neverTriggered2(r_3), neverTriggered2(r_3_1) }
+        (((r_3 != r_3_1 && s[r_3]) && s[r_3_1]) && NoPerm < sWildcard) && NoPerm < sWildcard ==> r_3 != r_3_1
+      );
+    
+    // -- check if sufficient permission is held
+      assert {:msg "  Exhale might fail. There might be insufficient permission to access r.f (test.vpr@14.11--14.12) [9]"}
+        (forall r_3: Ref ::
+        { Heap[r_3, f_6] } { QPMask[r_3, f_6] } { s[r_3] }
+        s[r_3] ==> Mask[r_3, f_6] > NoPerm || BMask[r_3, f_6]
+      );
+    
+    // -- assumptions for inverse of receiver r
+      assume (forall r_3: Ref ::
+        { Heap[r_3, f_6] } { QPMask[r_3, f_6] } { s[r_3] }
+        s[r_3] ==> qpRange2(r_3) && invRecv2(r_3) == r_3
+      );
+      assume (forall o_2: Ref ::
+        { invRecv2(o_2) }
+        s[invRecv2(o_2)] && qpRange2(o_2) ==> invRecv2(o_2) == o_2
+      );
+    
+    // -- assume permission updates for field f
+      assume (forall o_2: Ref ::
+        { QPMask[o_2, f_6] } { QPBMask[o_2, f_6] }
+        (s[invRecv2(o_2)] && qpRange2(o_2) ==> invRecv2(o_2) == o_2 && (QPMask[o_2, f_6] == Mask[o_2, f_6] && QPBMask[o_2, f_6] == BMask[o_2, f_6])) && (!(s[invRecv2(o_2)] && qpRange2(o_2)) ==> QPMask[o_2, f_6] == Mask[o_2, f_6] && QPBMask[o_2, f_6] == BMask[o_2, f_6])
+      );
+    
+    // -- assume permission updates for independent locations
+      assume (forall <A, B> o_2: Ref, f_4: (Field A B) ::
+        { QPMask[o_2, f_4] } { QPBMask[o_2, f_4] }
+        f_4 != f_6 ==> Mask[o_2, f_4] == QPMask[o_2, f_4] && BMask[o_2, f_4] == QPBMask[o_2, f_4]
+      );
+    Mask := QPMask;
+    BMask := QPBMask;
+    // Finish exhale
+    havoc ExhaleHeap;
+    assume IdenticalOnKnownLocations(Heap, ExhaleHeap, Mask, BMask);
+    Heap := ExhaleHeap;
     assume state(Heap, Mask, BMask);
 }
